The exponential generating function (egf) for sequence $\{a_n\}$ is $F(x)=**\sum_{n=0}^{\infty}a_n\frac{x^n}{n!}**$. 

Let $F(x)=\sum_{n=0}^{\infty}a_{n}\frac{x^{n}}{n!}$, $G(x)=\sum\frac{b_{n}x^{n}}{n!}$. Then $F(x)\cdot G(x)=**\sum c_{n}\frac{x^{n}}{n!},c_{n}=\sum_{i=0}^{n}\binom{n}{i}a_{i}b_{n-i}**$
> Let $a_{n}=\frac{\overline{a_{n}}}{n!},b_{n}=\frac{\overline{b_{n}}}{n!}$. 
> By the product of series: $c_{n}=\sum_{i=0}^{n}\frac{a_{i}}{i!}\frac{b_{n-i}}{(n-i)!}$
> Multiplying by $\frac{n!}{n!}$ $=\frac{1}{n!}\sum\frac{n!}{i!(n-i)!}a_{i}b_{n-i}$ $=\frac{1}{n!}\sum_{i=0}^{n}\binom{n}{i}a_{i}b_{n-i}$

***

