Inclusion-Exclusion Theorem: 
Let $A_1, \ldots A_n \subseteq X$, with all $A_i$'s being non-empty. Let $I \subseteq [n] = \{1, 2, \ldots n\}$, and denote $A_I = \cap_{i\in I}A_i$. Define $A_\emptyset = X$ (universal set). Then $|\cup_{i=1}^n A_i|=|X| - \sum_{I \subseteq [n]}(-1)^{|I|}|A_I|$ $\iff$ (DeMorgan's) $|\cap_{i=1}^nA_i| = \sum_{I\subseteq[n]}(-1)^{|I|}|A_I|$
> Ex: let $n = 2$, so $I = \emptyset, \{1\}, \{2\}, \{1, 2\}$ 
> So $|\cup_{i=1}^2 A_i| = |A_1 \cup A_2| = |X| - [|X| + (-1)^1 |A_{\{1\}}|+(-1)^1|A_{\{2\}}|] + (-1)^2 |A_{\{1, 2\}}|$
> $= |A_1| + |A_2| - |A_1 \cap A_2|$
> +
> Ex: Determine the total integer solutions to $x_1 + x_2 + x_3 = 35$, $0 \leq x_1, x_2, x_3 \leq 15$
> Here, $X$ denotes all weak compositions of $35$ into $3$ parts.
> +
> Solution:
> Let $A_{1}=\{\textrm{integer sol to } x_{1}+x_{2}+x_{3}=35\} = \{x_1 \geq 16; x_2, x_3 \geq 0 \}$ (weak composition of 19)
> Let $A_{3}=\{\textrm{integer sol to } x_{1}+x_{2}+x_{3}=35\} = \{x_2 \geq 16; x_1, x_3 \geq 0 \}$ 
> Let $A_{3}=\{\textrm{integer sol to } x_{1}+x_{2}+x_{3}=35\} = \{x_3 \geq 16; x_1, x_2 \geq 0 \}$ 
> We want $|A_1 \cup A_2 \cup A_3| = |\cap^3_{i=1}A_i| = \sum^{I \subseteq [3]}(-1)^{|I|}|A_I|$
> $=\binom{35 + 3 - 1}{3 - 1} + (-1)^1 \binom{3}{1}\binom{19 + 3 - 1}{3 - 1} + (-1)^2\binom{3}{2}\binom{3 + 3 - 1}{3 - 1}$ (weak composition of $35-2(16)=3$; $|A_1 \cap A_2|$) (first term is $0$) 
> +
> Ex:
> The Euler totient function $\phi(n)$ is the total number of values in the set $[n]$ that are relatively prime to $n$. 
> $\phi(6) = 2$ since $\textrm{GCD}(1,6) = 1$ and $\textrm{GCD}(5,6) = 1$. Let $n = p_1^{e_1} p_2^{e_2} \ldots p_t^{e_t}, e_i \geq 1$ for $i \leq i \leq t$ be the prime factorization. 
> +
> Solution:
> We want $\phi(n) = |\cap^t_{i=1}A_i| = \sum (-1)^{|I|}|A_I|$. 
> Let $A_i = \{a \in [n] : p_i \textrm{~divides~} a\} \subseteq n$
> Then $\phi(n) = |\cap_{i=1}^tA_i| = \sum_{i \subseteq[t]}(-1)^{|I|}|A_I|$
> $= n - [\frac{n}{p_1} + \frac{n}{p_2} + \ldots + \frac{n}{p_t}] + [\frac{n}{p_1p_2} + \frac{n}{p_1p_3} + \ldots] - [\frac{n}{p_1p_2p_3} + \ldots]$
> To understand this, brute force out a case; say $n = 100$, $p=5$, $|A_1| = ???$
> $=n[1 - \sum^t_{i=1}\frac{1}{p_i} + \sum_{i \leq i \leq j \leq t}\frac{1}{p_ip_j} - \sum_{i \leq i \leq j \leq k \leq t}\frac{1}{p_ip_jp_k}+\ldots]$
> $= n [(1 - \frac{1}{p_1})(1 - \frac{1}{p_2})(1 - \frac{1}{p_3})\ldots(1 - \frac{1}{p_t})]$
> $=n \prod\limits^{t}_{i=1}(1-\frac{1}{p_i})$ 
>+
>Let $A_i = \{f | f(j) \neq i \textrm{~for all~} j \in [n]\}$
>We want total surjective functions $= |\cap_{i=1}^kA_i|$
>$=\sum_{I \subseteq [k]} (-1)^{|I|} |A_I| = \sum^k_{i=0}(-1)^i \binom{k}{i} (k - i)^n$ ($f$ do NOT map to some values)
>$=k! S(n, k)$
>$\implies S(n,k) = \frac{1}{k!}\sum^{k}_{i=0}(-1)^k\binom{k}{i}(k-i)^n$, proving the formula from earlier

