Let $\{ a_{n}\}_{n\geq0}$ be a sequence. The formal power series **$F(x)=\sum_{n=0}^{\infty}a_{n}x^{n}$** is called the **ordinary generating function (OGF)** of $\{ a_{n}\}_{n\geq0}$.
> Example: Let $\{a_n\}_{n\geq0}$ be given by $\frac1{2!},\frac1{3!},\frac1{4!},\ldots$.
> Solution: 
> $\begin{aligned}\Rightarrow F(x)&=\frac{1}{2}+\frac{1}{2!}x+\frac{1}{4!}x^{2}+\ldots\\&=\frac{1}{x^{2}}(\frac{1}{2!}x^{2}+\frac{1}{3!}x^{3}+\frac{1}{4!}x^{4}+\ldots)\\&=\frac{1}{x^{2}}(\sum_{n=1}^{\infty}\frac{x^{n}}{n!})\end{aligned}$
> Thus $\frac1{x^2}(e^x-x-1)$ yields a closed form OGF for the sequence
> +
> Example: (opposite direction) Determine the sequence $\{a_n\}$ corresponding to OGF $F(x)=\sum a_{n}x^{n}=\frac{-4x+3}{(1-x)(1-2x)}$
> Solution:
> $\Rightarrow\frac{-4x+3}{(1-x)(1-2x)}=\frac{A}{1-x}+\frac{B}{1-2x}$
> $=\frac{1}{1-x}+\frac{2}{1-2x}$
> $=\sum_{n=0}^{\infty}x^n+\sum_{n=0}^{\infty}(2x)^n$
> $=\sum_{n=0}^{\infty}\left(1+2^{n+1}\right)x^{n}$
> $\Rightarrow\{a_n\}=\{1+2^{n-1}\}_{n\geq0}$

 
